type_system/declarational.v
@@ -13,18 +13,18 @@ Fixpoint handle_t Γ_len Z_len h T :=
   match T with
   | TApp n v => App (Var (Γ_len+n)) v
   | TAbsurd v => Absurd v
-  | TΠMatch v T => 
-      ΠMatch v (handle_t (2+Γ_len) Z_len h T)
-  | TΣMatch v T1 T2 => 
-      ΣMatch v
+  | TProdMatch v T => 
+      ProdMatch v (handle_t (2+Γ_len) Z_len h T)
+  | TSumMatch v T1 T2 => 
+      SumMatch v
         (handle_t (1+Γ_len) Z_len h T1) 
         (handle_t (1+Γ_len) Z_len h T2)
   | TListMatch v T1 T2 =>
       ListMatch v
         (handle_t Γ_len Z_len h T1)
         (handle_t (2+Γ_len) Z_len h T2)
-  | TLetBind c T =>
-      DoBind c (handle_t (1+Γ_len) Z_len h T)
+  | TDo c T =>
+      Do c (handle_t (1+Γ_len) Z_len h T)
   | TOp op v T =>
       match get_case h op with 
       | Some c_op =>
@@ -41,18 +41,18 @@ Fixpoint tmpl_to_comp Γ_len T :=
   match T with
   | TApp n v => App (Var (Γ_len+n)) v
   | TAbsurd v => Absurd v
-  | TΠMatch v T => 
-      ΠMatch v (tmpl_to_comp (2+Γ_len) T)
-  | TΣMatch v T1 T2 => 
-      ΣMatch v
+  | TProdMatch v T => 
+      ProdMatch v (tmpl_to_comp (2+Γ_len) T)
+  | TSumMatch v T1 T2 => 
+      SumMatch v
         (tmpl_to_comp (1+Γ_len) T1) 
         (tmpl_to_comp (1+Γ_len) T2)
   | TListMatch v T1 T2 => 
       ListMatch v
         (tmpl_to_comp Γ_len T1) 
         (tmpl_to_comp (2+Γ_len) T2)
-  | TLetBind c T =>
-      DoBind c (tmpl_to_comp (1+Γ_len) T)
+  | TDo c T =>
+      Do c (tmpl_to_comp (1+Γ_len) T)
   | TOp op v T =>
       Op op v (tmpl_to_comp (1+Γ_len) T)
   end.
@@ -62,9 +62,9 @@ Fixpoint tmpl_to_comp Γ_len T :=
 Inductive wf_vtype : vtype -> Prop :=
 | WfTyUnit : wf_vtype TyUnit 
 | WfTyInt : wf_vtype TyInt
-| WfTyEmpty : wf_vtype TyØ
-| WfTyΣ A B: wf_vtype A -> wf_vtype B -> wf_vtype (TyΣ A B)
-| WfTyΠ A B : wf_vtype A -> wf_vtype B -> wf_vtype (TyΠ A B)
+| WfTyEmpty : wf_vtype TyEmpty
+| WfTySum A B: wf_vtype A -> wf_vtype B -> wf_vtype (TySum A B)
+| WfTyProd A B : wf_vtype A -> wf_vtype B -> wf_vtype (TyProd A B)
 | WfTyList A : wf_vtype A -> wf_vtype (TyList A)
 | WfTyFun A C : wf_vtype A -> wf_ctype C -> wf_vtype (TyFun A C)
 | WfTyHandler C D : wf_ctype C -> wf_ctype D -> wf_vtype (TyHandler C D)
@@ -92,23 +92,23 @@ with wf_t : ctx -> tctx -> tmpl -> sig -> Prop :=
     has_vtype Γ v A -> get_ttype Z n = Some A ->
     wf_t Γ Z (TApp n v) Σ
 | WfTAbsurd Γ Z v Σ :
-    has_vtype Γ v TyØ -> 
+    has_vtype Γ v TyEmpty -> 
     wf_t Γ Z (TAbsurd v) Σ 
-| WfTΠMatch Γ Z v T A B Σ :
-    has_vtype Γ v (TyΠ A B) -> wf_t (CtxU (CtxU Γ A) B) Z T Σ -> 
-    wf_t Γ Z (TΠMatch v T) Σ
-| WfTΣMatch Γ Z v T1 T2 A B Σ :
-    has_vtype Γ v (TyΣ A B) -> 
+| WfTProdMatch Γ Z v T A B Σ :
+    has_vtype Γ v (TyProd A B) -> wf_t (CtxU (CtxU Γ A) B) Z T Σ -> 
+    wf_t Γ Z (TProdMatch v T) Σ
+| WfTSumMatch Γ Z v T1 T2 A B Σ :
+    has_vtype Γ v (TySum A B) -> 
     wf_t (CtxU Γ A) Z T1 Σ -> wf_t (CtxU Γ B) Z T2 Σ -> 
-    wf_t Γ Z (TΣMatch v T1 T2) Σ
+    wf_t Γ Z (TSumMatch v T1 T2) Σ
 | WfTListMatch Γ Z v T1 T2 A Σ :
     has_vtype Γ v (TyList A) -> 
     wf_t Γ Z T1 Σ -> wf_t (CtxU (CtxU Γ A) (TyList A)) Z T2 Σ ->  
     wf_t Γ Z (TListMatch v T1 T2) Σ
-| WfTLetBind Γ Z c T A Σ :
+| WfTDo Γ Z c T A Σ :
     has_ctype Γ c (CTy A SigØ EqsØ) ->
     wf_t (CtxU Γ A) Z T Σ ->
-    wf_t  Γ Z (TLetBind c T) Σ
+    wf_t  Γ Z (TDo c T) Σ
 | WfTOp Γ Z op v T Aop Bop Σ :
     get_op_type Σ op = Some (Aop, Bop) -> has_vtype Γ v Aop ->
     wf_t (CtxU Γ Bop) Z T Σ ->
@@ -140,19 +140,19 @@ with has_vtype' : ctx -> val -> vtype -> Prop :=
 | TypePair Γ v1 v2 A B :
     has_vtype Γ v1 A ->
     has_vtype Γ v2 B ->
-    has_vtype' Γ (Pair v1 v2) (TyΠ A B)
-| TypeInl Γ v A B :
+    has_vtype' Γ (Pair v1 v2) (TyProd A B)
+| TypeLeft Γ v A B :
     has_vtype Γ v A ->
-    has_vtype' Γ (Inl v) (TyΣ A B)
-| TypeInr Γ v A B :
+    has_vtype' Γ (Left v) (TySum A B)
+| TypeRight Γ v A B :
     has_vtype Γ v B ->
-    has_vtype' Γ (Inr v) (TyΣ A B)
-| TypeListNil Γ A :
-    has_vtype' Γ ListNil (TyList A)
-| TypeListCons Γ v vs A :
+    has_vtype' Γ (Right v) (TySum A B)
+| TypeNil Γ A :
+    has_vtype' Γ Nil (TyList A)
+| TypeCons Γ v vs A :
     has_vtype Γ v A ->
     has_vtype Γ vs (TyList A) ->
-    has_vtype' Γ (ListCons v vs) (TyList A)
+    has_vtype' Γ (Cons v vs) (TyList A)
 | TypeFun Γ c A C :
     has_ctype (CtxU Γ A) c C ->
     has_vtype' Γ (Fun c) (TyFun A C)
@@ -161,7 +161,7 @@ with has_vtype' : ctx -> val -> vtype -> Prop :=
     has_htype Γ h Σ D -> 
     respects Γ h Σ D E ->
     has_vtype' Γ (Handler cr h) (TyHandler (CTy A Σ E) D)
-| TypeVSubtype Γ v A A' :
+| TypeVSubsume Γ v A A' :
     has_vtype Γ v A ->
     vsubtype A A' -> 
     has_vtype' Γ v A'
@@ -177,26 +177,26 @@ with has_ctype' : ctx -> comp -> ctype -> Prop :=
     has_vtype Γ v A ->
     has_ctype' Γ (Ret v) (CTy A SigØ EqsØ)
 | TypeAbsurd Γ v C :
-    has_vtype Γ v TyØ -> 
+    has_vtype Γ v TyEmpty -> 
     has_ctype' Γ (Absurd v) C
-| TypeΠMatch Γ v A B c C :
-    has_vtype Γ v (TyΠ A B) ->
+| TypeProdMatch Γ v A B c C :
+    has_vtype Γ v (TyProd A B) ->
     has_ctype (CtxU (CtxU Γ A) B) c C ->
-    has_ctype' Γ (ΠMatch v c) C
-| TypeΣMatch Γ v A B c1 c2 C :
-    has_vtype Γ v (TyΣ A B) ->
+    has_ctype' Γ (ProdMatch v c) C
+| TypeSumMatch Γ v A B c1 c2 C :
+    has_vtype Γ v (TySum A B) ->
     has_ctype (CtxU Γ A) c1 C ->
     has_ctype (CtxU Γ B) c2 C ->
-    has_ctype' Γ (ΣMatch v c1 c2) C
+    has_ctype' Γ (SumMatch v c1 c2) C
 | TypeListMatch Γ v A c1 c2 C :
     has_vtype Γ v (TyList A) ->
     has_ctype Γ c1 C ->
     has_ctype (CtxU (CtxU Γ A) (TyList A)) c2 C ->
     has_ctype' Γ (ListMatch v c1 c2) C
-| TypeDoBind Γ c1 c2 A B Σ E :
+| TypeDo Γ c1 c2 A B Σ E :
     has_ctype Γ c1 (CTy A Σ E) ->
     has_ctype (CtxU Γ A) c2 (CTy B Σ E) ->
-    has_ctype' Γ (DoBind c1 c2) (CTy B Σ E)
+    has_ctype' Γ (Do c1 c2) (CTy B Σ E)
 | TypeApp Γ v1 v2 A C :
     has_vtype Γ v1 (TyFun A C) ->
     has_vtype Γ v2 A ->
@@ -214,7 +214,7 @@ with has_ctype' : ctx -> comp -> ctype -> Prop :=
     has_vtype Γ v Aop ->
     has_ctype (CtxU Γ Bop) c (CTy A Σ E) ->
     has_ctype' Γ (Op op v c) (CTy A Σ E)
-| TypeCSubtype Γ c C C' :
+| TypeCSubsume Γ c C C' :
     has_ctype Γ c C -> 
     csubtype C C' -> 
     has_ctype' Γ c C'
@@ -273,19 +273,19 @@ with veq': vtype -> ctx -> val -> val -> Prop :=
 | VeqPair A B Γ v1 v1' v2 v2' :
     veq A Γ v1 v1' ->
     veq B Γ v2 v2' -> 
-    veq' (TyΠ A B) Γ (Pair v1 v2) (Pair v1' v2')
-| VeqInl A B Γ v v' :
+    veq' (TyProd A B) Γ (Pair v1 v2) (Pair v1' v2')
+| VeqLeft A B Γ v v' :
     veq A Γ v v' ->
-    veq' (TyΣ A B) Γ (Inl v) (Inl v')
-| VeqInr A B Γ v v' :
+    veq' (TySum A B) Γ (Left v) (Left v')
+| VeqRight A B Γ v v' :
     veq B Γ v v' ->
-    veq' (TyΣ A B) Γ (Inr v) (Inr v')
-| VeqListNil A Γ :
-    veq' (TyList A) Γ ListNil ListNil
-| VeqListCons A Γ v v' vs vs':
+    veq' (TySum A B) Γ (Right v) (Right v')
+| VeqNil A Γ :
+    veq' (TyList A) Γ Nil Nil
+| VeqCons A Γ v v' vs vs':
     veq A Γ v v' ->
     veq (TyList A) Γ vs vs' ->
-    veq' (TyList A) Γ (ListCons v vs) (ListCons v' vs')
+    veq' (TyList A) Γ (Cons v vs) (Cons v' vs')
 | VeqFun A C Γ c c':
     ceq C (CtxU Γ A) c c' ->
     veq' (TyFun A C) Γ (Fun c) (Fun c')
@@ -319,24 +319,24 @@ with ceq' : ctype -> ctx -> comp -> comp -> Prop :=
     ceq' (CTy A Σ E) Γ (Ret v) (Ret v')
 | CeqAbsurd C Γ v v' :
     ceq' C Γ (Absurd v) (Absurd v')
-| CeqΠMatch Γ C v v' A B c c':
-    veq (TyΠ A B) Γ v v' ->
+| CeqProdMatch Γ C v v' A B c c':
+    veq (TyProd A B) Γ v v' ->
     ceq C (CtxU (CtxU Γ A) B) c c' ->
-    ceq' C Γ (ΠMatch v c) (ΠMatch v' c')
-| CeqΣMatch Γ C v v' A B c1 c1' c2 c2':
-    veq (TyΣ A B) Γ v v' ->
+    ceq' C Γ (ProdMatch v c) (ProdMatch v' c')
+| CeqSumMatch Γ C v v' A B c1 c1' c2 c2':
+    veq (TySum A B) Γ v v' ->
     ceq C (CtxU Γ A) c1 c1' ->
     ceq C (CtxU Γ B) c2 c2' ->
-    ceq' C Γ (ΣMatch v c1 c2) (ΣMatch v' c1' c2')
+    ceq' C Γ (SumMatch v c1 c2) (SumMatch v' c1' c2')
 | CeqListMatch Γ C v v' A c1 c1' c2 c2':
     veq (TyList A) Γ v v' ->
     ceq C Γ c1 c1' ->
     ceq C (CtxU (CtxU Γ A) (TyList A)) c2 c2' ->
     ceq' C Γ (ListMatch v c1 c2) (ListMatch v' c1' c2')
-| CeqDoBind A B Σ E Γ c1 c1' c2 c2':
+| CeqDo A B Σ E Γ c1 c1' c2 c2':
     ceq (CTy A Σ E) Γ c1 c1' ->
     ceq (CTy B Σ E) (CtxU Γ A) c2 c2' ->
-    ceq' (CTy B Σ E) Γ (DoBind c1 c2) (DoBind c1' c2')
+    ceq' (CTy B Σ E) Γ (Do c1 c2) (Do c1' c2')
 | CeqApp Γ v1 v1' v2 v2' A C:
     veq (TyFun A C) Γ v1 v1' ->
     veq A Γ v2 v2' ->
@@ -360,25 +360,25 @@ with ceq' : ctype -> ctx -> comp -> comp -> Prop :=
     c_inst (tmpl_to_comp (ctx_len Γ) T1) I = c1 ->
     c_inst (tmpl_to_comp (ctx_len Γ) T2) I = c2 ->
     ceq' (CTy A Σ E) Γ' c1 c2
-| βΠMatch v1 v2 c C Γ: 
+| βMatchPair v1 v2 c C Γ: 
     ceq' C Γ
-      (ΠMatch (Pair v1 v2) c) 
+      (ProdMatch (Pair v1 v2) c) 
       (c_subs2_out c v1 v2)
-| βΣMatch_Inl v c1 c2 C Γ:
+| βMatchLeft v c1 c2 C Γ:
     ceq' C Γ
-      (ΣMatch (Inl v) c1 c2)
+      (SumMatch (Left v) c1 c2)
       (c_subs_out c1 v)
-| βΣMatch_Inr v c1 c2 C Γ:
+| βMatchRight v c1 c2 C Γ:
     ceq' C Γ 
-      (ΣMatch (Inr v) c1 c2)
+      (SumMatch (Right v) c1 c2)
       (c_subs_out c2 v)
-| βListMatch_Nil c1 c2 C Γ:
+| βMatchNil c1 c2 C Γ:
     ceq' C Γ
-      (ListMatch ListNil c1 c2)
+      (ListMatch Nil c1 c2)
       c1
-| βListMatch_Cons v vs c1 c2 C Γ:
+| βMatchCons v vs c1 c2 C Γ:
     ceq' C Γ
-      (ListMatch (ListCons v vs) c1 c2)
+      (ListMatch (Cons v vs) c1 c2)
       (c_subs2_out c2 v vs)
 | βApp c v C Γ:
     ceq' C Γ (App (Fun c) v) (c_subs_out c v)
@@ -386,17 +386,17 @@ with ceq' : ctype -> ctx -> comp -> comp -> Prop :=
     ceq' C Γ
       (LetRec c1 c2)
       (c_subs_out c2 (Fun (LetRec (c_shift c1 1 2) c1)))
-| βDoBind_Ret v c C Γ:
-    ceq' C Γ (DoBind (Ret v) c) (c_subs_out c v)
-| βDoBind_Op op v c1 c2 C Γ:
+| βDoRet v c C Γ:
+    ceq' C Γ (Do (Ret v) c) (c_subs_out c v)
+| βDoOp op v c1 c2 C Γ:
     ceq' C Γ
-      (DoBind (Op op v c1) c2)
-      (Op op v (DoBind c1 (c_shift c2 1 1)))
-| βHandle_Ret c_r h v C Γ:
+      (Do (Op op v c1) c2)
+      (Op op v (Do c1 (c_shift c2 1 1)))
+| βHandleRet c_r h v C Γ:
     ceq' C Γ
       (Handle (Handler c_r h) (Ret v))
       (c_subs_out c_r v)
-| βHandle_Op c_r h op v c_k c_op C Γ:
+| βHandleOp c_r h op v c_k c_op C Γ:
     get_case h op = Some c_op ->
     ceq' C Γ
       (Handle (Handler c_r h) (Op op v c_k))
@@ -405,29 +405,29 @@ with ceq' : ctype -> ctx -> comp -> comp -> Prop :=
         v )
 | ηEmpty Γ v n c C:
     n <= ctx_len Γ ->
-    has_ctype (ctx_insert Γ n (TyØ)) c C ->
+    has_ctype (ctx_insert Γ n (TyEmpty)) c C ->
     ceq' C Γ (c_subs c n v) (Absurd v)
 | ηPair Γ v n c C A B:
     n <= ctx_len Γ ->
-    has_ctype (ctx_insert Γ n (TyΠ A B)) c C ->
+    has_ctype (ctx_insert Γ n (TyProd A B)) c C ->
     ceq' C Γ (c_subs c n v)
-      (ΠMatch v (c_subs (c_shift c 2 0) (2+n) (Pair (Var 1) (Var 0))))
+      (ProdMatch v (c_subs (c_shift c 2 0) (2+n) (Pair (Var 1) (Var 0))))
 | ηSum Γ v n c C A B:
     n <= ctx_len Γ ->
-    has_ctype (ctx_insert Γ n (TyΣ A B)) c C ->
+    has_ctype (ctx_insert Γ n (TySum A B)) c C ->
     ceq' C Γ (c_subs c n v) 
-      (ΣMatch v 
-        (c_subs (c_shift c 1 0) (1+n) (Inl (Var 0))) 
-        (c_subs (c_shift c 1 0) (1+n) (Inr (Var 0))))
+      (SumMatch v 
+        (c_subs (c_shift c 1 0) (1+n) (Left (Var 0))) 
+        (c_subs (c_shift c 1 0) (1+n) (Right (Var 0))))
 | ηList Γ v n c C A:
     n <= ctx_len Γ ->
     has_ctype (ctx_insert Γ n (TyList A)) c C ->
     ceq' C Γ (c_subs c n v) 
       (ListMatch v 
-        (c_subs c n ListNil) 
-        (c_subs (c_shift c 2 0) (2+n) (ListCons (Var 1) (Var 0))))
-| ηDoBind Γ c C:
-    ceq' C Γ (DoBind c (Ret (Var 0))) c
+        (c_subs c n Nil) 
+        (c_subs (c_shift c 2 0) (2+n) (Cons (Var 1) (Var 0))))
+| ηDo Γ c C:
+    ceq' C Γ (Do c (Ret (Var 0))) c
 
 with heq : sig -> ctype -> ctx -> hcases -> hcases -> Prop :=
 | Heq Σ Σ1 Σ2 D Γ h1 h2 : 
